examples/Tauto/Tauto.v
@@ -3,11 +3,6 @@ Require Import Coq.Bool.Bool.
 
 Require Import ExtLib.Core.RelDec.
 
-Require Import McExamples.Tauto.MSimpleTyp.
-Require Import McExamples.Tauto.ILogic.
-Require Import McExamples.Tauto.ILogicFunc.
-Require Import McExamples.Tauto.ILogicReify.
-
 Require Import MirrorCore.Lambda.Red.
 Require Import MirrorCore.MTypes.ModularTypes.
 Require Import MirrorCore.Lambda.ExprCore.
@@ -18,10 +13,17 @@ Require Import MirrorCore.Polymorphic.
 Require Import MirrorCore.Lambda.ExprUnify_simple.
 Require Import MirrorCore.RTac.RTac.
 
+
+Require Import McExamples.Tauto.MSimpleTyp.
+Require Import McExamples.Tauto.ILogic.
+Require Import McExamples.Tauto.ILogicFunc.
+Require Import McExamples.Tauto.ILogicReify.
+
+
 Definition tc (t : typ) :=
   match t with
-    | ModularTypes.tyProp => true
-    | _ => false
+  | ModularTypes.tyProp => true
+  | _ => false
   end.
 
 Require Import MirrorCore.Reify.Reify.
@@ -31,15 +33,12 @@ Definition test : (lemma typ (expr typ ilfunc) (expr typ ilfunc)) :=
   Eval unfold Lemma.add_var, Lemma.add_prem , Lemma.vars , Lemma.concl , Lemma.premises in
   <:: @limplAdj Prop _ _ ::>.
 
-Print test.
-Check limplAdj.
-
 Definition conclD (us vs : tenv typ) (e : expr typ ilfunc) : option (exprT us vs Prop) :=
   exprD us vs tyProp e.
 
 Definition r_refl : PolyLemma typ (expr typ ilfunc) (expr typ ilfunc) :=
   {| p_n := 1;
-     p_lem := fun t => 
+     p_lem := fun t =>
                {| vars := t :: nil;
                   premises := nil;
                   concl := App (App (Inj (fEntails t)) (Var 0)) (Var 0) |};
@@ -56,7 +55,7 @@ Qed.
 
 Definition r_trueR : PolyLemma typ (expr typ ilfunc) (expr typ ilfunc) :=
   {| p_n := 1;
-     p_lem := fun t => 
+     p_lem := fun t =>
                {| vars := t :: nil;
                   premises := nil;
                   concl := App (App (Inj (fEntails t)) (Var 0)) (mkTrue t) |};
@@ -75,7 +74,7 @@ Qed.
 
 Definition r_falseL : PolyLemma typ (expr typ ilfunc) (expr typ ilfunc) :=
   {| p_n := 1;
-     p_lem := fun t => 
+     p_lem := fun t =>
                {| vars := t :: nil;
                   premises := nil;
                   concl := App (App (Inj (fEntails t)) (mkFalse t)) (Var 0) |};
@@ -84,7 +83,7 @@ Definition r_falseL : PolyLemma typ (expr typ ilfunc) (expr typ ilfunc) :=
 
 Definition r_andR : PolyLemma typ (expr typ ilfunc) (expr typ ilfunc) :=
   {| p_n := 1;
-     p_lem := fun t => 
+     p_lem := fun t =>
                {| vars := t :: t :: t :: nil;
                   premises := App (App (Inj (fEntails t)) (Var 0)) (Var 2)
                                   :: App (App (Inj (fEntails t)) (Var 0)) (Var 1) :: nil;
@@ -95,7 +94,7 @@ Definition r_andR : PolyLemma typ (expr typ ilfunc) (expr typ ilfunc) :=
 
 Definition r_andL1 : PolyLemma typ (expr typ ilfunc) (expr typ ilfunc) :=
   {| p_n := 1;
-     p_lem := fun t => 
+     p_lem := fun t =>
                {| vars := t :: t :: t :: nil;
                   premises := App (App (Inj (fEntails t)) (Var 2))
                                   (Var 0) :: nil;
@@ -108,7 +107,7 @@ Definition r_andL1 : PolyLemma typ (expr typ ilfunc) (expr typ ilfunc) :=
 
 Definition r_andL2 : PolyLemma typ (expr typ ilfunc) (expr typ ilfunc) :=
   {| p_n := 1;
-     p_lem := fun t => 
+     p_lem := fun t =>
                {| vars := t :: t :: t :: nil;
                   premises := App (App (Inj (fEntails t)) (Var 1))
                                   (Var 0) :: nil;
@@ -121,7 +120,7 @@ Definition r_andL2 : PolyLemma typ (expr typ ilfunc) (expr typ ilfunc) :=
 
 Definition r_orL : PolyLemma typ (expr typ ilfunc) (expr typ ilfunc) :=
   {| p_n := 1;
-     p_lem := fun t => 
+     p_lem := fun t =>
                {| vars := t :: t :: t :: nil;
                   premises := App (App (Inj (fEntails t)) (Var 2))
                                   (Var 0)
@@ -136,7 +135,7 @@ Definition r_orL : PolyLemma typ (expr typ ilfunc) (expr typ ilfunc) :=
 
 Definition r_orR1 : PolyLemma typ (expr typ ilfunc) (expr typ ilfunc) :=
   {| p_n := 1;
-     p_lem := fun t => 
+     p_lem := fun t =>
                {| vars := t :: t :: t :: nil;
                   premises := App (App (Inj (fEntails t)) (Var 0))
                                   (Var 2) :: nil;
@@ -147,7 +146,7 @@ Definition r_orR1 : PolyLemma typ (expr typ ilfunc) (expr typ ilfunc) :=
 
 Definition r_orR2 : PolyLemma typ (expr typ ilfunc) (expr typ ilfunc) :=
   {| p_n := 1;
-     p_lem := fun t => 
+     p_lem := fun t =>
                {| vars := t :: t :: t :: nil;
                   premises := App (App (Inj (fEntails t)) (Var 0))
                                   (Var 1) :: nil;
@@ -158,7 +157,7 @@ Definition r_orR2 : PolyLemma typ (expr typ ilfunc) (expr typ ilfunc) :=
 
 Definition r_implAdj : PolyLemma typ (expr typ ilfunc) (expr typ ilfunc) :=
   {| p_n := 1;
-     p_lem := fun t => 
+     p_lem := fun t =>
                {| vars := t :: t :: t :: nil;
                   premises := App
                                 (App (Inj (fEntails t))
@@ -169,12 +168,11 @@ Definition r_implAdj : PolyLemma typ (expr typ ilfunc) (expr typ ilfunc) :=
      p_tc := tc
   |}.
 
-
 Definition PAPPLY (plem : PolyLemma typ (expr typ ilfunc) (expr typ ilfunc)) :=
-  PAPPLY 
+  PAPPLY
     (fun subst SS SU tus tvs n l r t s =>
               @exprUnify subst typ ilfunc RType_typ RSym_ilfunc Typ2_Fun
-                         SS SU 10 tus tvs n l r t s) plem.
+                         SS SU 10 tus tvs n l r t s) ilfunc_unify plem.
 
 Definition fintro (e : expr typ ilfunc) : option (@OpenAs typ (expr typ ilfunc)) :=
   match e with
@@ -207,37 +205,26 @@ Definition INTRO := @INTRO typ (expr typ ilfunc) ExprVar_expr ExprUVar_expr fint
 Definition TAUTO : rtac typ (expr typ ilfunc) :=
   REC 10
       (fun r =>
-         THEN (REPEAT 10 INTRO) 
-              (runOnGoals 
+         THEN (REPEAT 10 INTRO)
+              (runOnGoals
                  (FIRST
                     (PAPPLY r_trueR ::
-                     PAPPLY r_falseL :: 
-                     PAPPLY r_refl :: 
-                     THEN (PAPPLY r_andR) (runOnGoals r) :: 
-                     THEN (PAPPLY r_orL) (runOnGoals r) :: 
-                     SOLVE (THEN (PAPPLY r_orR1) (runOnGoals r)) :: 
-                     SOLVE (THEN (PAPPLY r_orR2) (runOnGoals r)) :: 
-                     SOLVE (THEN (PAPPLY r_andL1) (runOnGoals r)) :: 
+                     PAPPLY r_falseL ::
+                     PAPPLY r_refl ::
+                     THEN (PAPPLY r_andR) (runOnGoals r) ::
+                     THEN (PAPPLY r_orL) (runOnGoals r) ::
+                     SOLVE (THEN (PAPPLY r_orR1) (runOnGoals r)) ::
+                     SOLVE (THEN (PAPPLY r_orR2) (runOnGoals r)) ::
+                     SOLVE (THEN (PAPPLY r_andL1) (runOnGoals r)) ::
                      SOLVE (THEN (PAPPLY r_andL2) (runOnGoals r)) :: nil)))) FAIL.
 
 Goal True.
-  
-pose (PApply.get_lemma r_trueR
+
+pose (PApply.get_lemma ilfunc_unify r_trueR
                        (mkEntails tyProp (mkTrue tyProp) (mkTrue tyProp))).
 
 cbv beta zeta iota delta [PApply.get_lemma PolyInst.get_inst PolyInst.get_types PolyInst.get_vector PolyInst.build_vector PApply.view_update p_n p_lem p_tc Functor.fmap Functor_polymorphic fmap_polymorphic] in o.
 
 cbv beta zeta iota delta [r_trueR inst concl Functor.fmap Functor_polymorphic fmap_polymorphic mkTrue mkEntails Vector.vector_hd tc mkTrue mkEntails fTrue fEntails typeof_sym RSym_ilfunc typeof_ilfunc] in o.
-
-(* looks like maybe we are calling typeclass on
-   an uninstantiated thing? *)
-
-(* note that gs (tyVar 1) is what is failing. *)
-
-(* problem - tyVars aren't instantiated! *)
-
-compute in o.
-(* Gregory, I'm pretty sure this should be evaluate to Some *)
-
 apply I.
 Qed.
